Deploying to gh-pages from @ xubaiw/reservoir-index@9e67c115231e168dbd36334f2cb492bbc3543f16 🚀

git/g4rgoil/tba-project/TBA/While/Com.lean
@@ -1,70 +1,91 @@
 /- The com Language -/
 namespace While
 
+abbrev Map (α β : Type) := α → Option β
+
+namespace Map
+
+def empty : Map α β := λ _ => none
+
+def update [DecidableEq α] (m : Map α β) (k : α) (v : Option β) : Map α β :=
+  λ k' => if k = k' then v else m k'
+
+scoped notation:max m "[" k " ↦ " v "]" => update m k v
+
+end Map
+
 /- Variables and Values -/
 
 /-- names for variables -/
 abbrev VName := String
 
-inductive Val where
-  | bool (b : Bool)
-  | int  (i : Int)
+inductive Ty where
+  | int | bool
+  deriving DecidableEq
+
+inductive Val : Ty → Type where
+  | bool (b : Bool) : Val Ty.bool
+  | int  (i : Int)  : Val Ty.int
   deriving DecidableEq
 
 -- lets us use a `Bool/Int` where a `Val` is expected
-instance : Coe Bool Val := ⟨Val.bool⟩
-instance : Coe Int Val  := ⟨Val.int⟩
-#check (true : Val)
+instance : Coe Bool (Val Ty.bool) := ⟨Val.bool⟩
+instance : Coe Int  (Val Ty.int)  := ⟨Val.int⟩
 
 /- Expressions and Commands -/
 
+abbrev Ctxt := Map VName Ty
+
 /-- binary operations -/
-inductive BinOp where
-  | eq | and | lt | add | sub
+inductive BinOp : Ty → Ty → Type where
+  | eq  : BinOp τ     .bool
+  | and : BinOp .bool .bool
+  | lt  : BinOp .int  .bool
+  | add : BinOp .int  .int
+  | sub : BinOp .int  .int
 
-inductive Expr where
-  | const (v : Val)
-  | var (x : VName)
-  | binop (l : Expr) (op : BinOp) (r : Expr)
+inductive Expr : Ctxt → Ty → Type where
+  | const (v : Val τ) : Expr Γ τ
+  | var (x : VName) (h : Γ x = some τ) : Expr Γ τ
+  | binop (l : Expr Γ α) (op : BinOp α β) (r : Expr Γ α) : Expr Γ β
 
-instance : Coe Val   Expr := ⟨Expr.const⟩
-instance : Coe VName Expr := ⟨Expr.var⟩
+instance : Coe (Val τ) (Expr Γ τ) := ⟨Expr.const⟩
 
-def BinOp.eval : BinOp → Val → Val → Option Val
-  | BinOp.eq,  v₁,          v₂          => some (Val.bool (v₁ = v₂))
-  | BinOp.and, Val.bool b₁, Val.bool b₂ => some (Val.bool (b₁ ∧ b₂))
-  | BinOp.lt,  Val.int i₁,  Val.int i₂  => some (Val.bool (i₁ < i₂))
-  | BinOp.add, Val.int i₁,  Val.int i₂  => some (Val.int (i₁ + i₂))
-  | BinOp.sub, Val.int i₁,  Val.int i₂  => some (Val.int (i₁ - i₂))
-  | _,         _,           _           => none
+def BinOp.eval : BinOp α β → Val α → Val α → Val β
+  | BinOp.eq,        v₁,       v₂ => Val.bool (v₁ = v₂)
+  | BinOp.and, .bool b₁, .bool b₂ => Val.bool (b₁ ∧ b₂)
+  | BinOp.lt,  .int  i₁, .int  i₂ => Val.bool (i₁ < i₂)
+  | BinOp.add, .int  i₁, .int  i₂ => Val.int  (i₁ + i₂)
+  | BinOp.sub, .int  i₁, .int  i₂ => Val.int  (i₁ - i₂)
 
-inductive Com where
+inductive Com (Γ : Ctxt) where
   | skip
-  | ass (x : VName) (e : Expr)
-  | seq (c c' : Com)
-  | cond (b : Expr) (cₜ cₑ : Com)
-  -- `while` is already a keyword, so escape name using French quotes «...».
-  -- Note that in *expression contexts* (basically everywhere except at `induction/cases ... | «while» ...`),
-  -- `Com.while` or often simply `.while` is accepted without escaping.
-  | «while» (b : Expr) (c : Com)
+  | ass (x : VName) (e : Expr Γ τ) (h : Γ x = some τ)
+  | seq (c c' : Com Γ)
+  | cond (b : Expr Γ Ty.bool) (cₜ cₑ : Com Γ)
+  | «while» (b : Expr Γ Ty.bool) (c : Com Γ)
 
-open Com
+theorem Expr.bool_rec (p : Expr Γ Ty.bool → Prop)
+    (htrue : p true) (hfalse : p false) (hvar : ∀ x h, p (Expr.var x h))
+    (hbinop : ∀ α l op r, p (@Expr.binop _ α _ l op r)) : ∀ x, p x
+  | true | false | .var .. | .binop .. => by simp_all
 
-infix:150 " ::= " => ass
-infixr:130 ";; "  => seq
+
+infixr:130 ";; "  => Com.seq
 
 /- Prettier embedding of `Expr` and `Com` as term-level macros -/
 /- (You can ignore this part, jump to the examples below to see its usage) -/
 
 open Lean
+open Map
 
 syntax "`[Expr|" term "]" : term
 
 macro_rules
-  | `(`[Expr|true])     => `((true : Expr))
-  | `(`[Expr|false])    => `((false : Expr))
-  | `(`[Expr|$n:num])   => `((($n : Nat) : Expr))
-  | `(`[Expr|$x:ident]) => `(($(quote x.getId.toString) : Expr))
+  | `(`[Expr|true])     => `((true : Expr _ Ty.bool))
+  | `(`[Expr|false])    => `((false : Expr _ Ty.bool))
+  | `(`[Expr|$n:num])   => `((($n : Nat) : Expr _ Ty.int))
+  | `(`[Expr|$x:ident]) => `((Expr.var $(quote x.getId.toString) rfl : Expr _ _))
   | `(`[Expr|$x = $y])  => `(Expr.binop `[Expr|$x] BinOp.eq `[Expr|$y])
   | `(`[Expr|$x && $y]) => `(Expr.binop `[Expr|$x] BinOp.and `[Expr|$y])
   | `(`[Expr|$x < $y])  => `(Expr.binop `[Expr|$x] BinOp.lt `[Expr|$y])
@@ -74,6 +95,7 @@ macro_rules
 
 declare_syntax_cat com
 
+
 syntax ident " := " term ";\n" : com
 syntax "if " "(" term ")" " {\n" com* "\n}" (" else " "{\n" com* "\n}")? : com
 syntax "while " "(" term ")" " {\n" com* "\n}" : com
@@ -82,15 +104,36 @@ syntax "`[Com|" com* "]" : term
 
 macro_rules
   | `(`[Com|])                    => `(Com.skip)
-  | `(`[Com|$x:ident := $e;])     => `($(quote x.getId.toString) ::= `[Expr|$e])
+  | `(`[Com|$x:ident := $e;])     => `(Com.ass $(quote x.getId.toString) `[Expr|$e] rfl)
   | `(`[Com|if ($b) { $cts* } else { $cfs* }]) =>
     `(Com.cond `[Expr|$b] `[Com|$cts*] `[Com|$cfs*])
   | `(`[Com|if ($b) { $cts* }])   => `(`[Com|if ($b) { $cts* } else {}])
   | `(`[Com|while ($b) { $cs* }]) => `(Com.while `[Expr|$b] `[Com|$cs*])
   | `(`[Com|$c $cs*])             => `(Com.seq `[Com|$c] `[Com|$cs*])
 
+end While
 
-def example1 := `[Com|
+namespace test
+
+open While
+open Expr
+open Map
+
+abbrev Γ : Ctxt := Map.empty["x" ↦ Ty.int]["y" ↦ Ty.int]["b" ↦ Ty.bool]
+
+def e01 :  Expr Γ Ty.bool := `[Expr| true]
+def e02 :  Expr Γ Ty.bool := `[Expr| false]
+def e03 :  Expr Γ Ty.int  := `[Expr| 42]
+def e04a : Expr Γ Ty.int  := `[Expr| x]
+def e04b : Expr Γ Ty.bool := `[Expr| b]
+def e06 :  Expr Γ Ty.bool := `[Expr| 42 = 28]
+def e07 :  Expr Γ Ty.bool := `[Expr| true && false]
+def e08 :  Expr Γ Ty.bool := `[Expr| 0 < 1]
+def e09 :  Expr Γ Ty.int  := `[Expr| 1 + 1]
+def e10 :  Expr Γ Ty.int  := `[Expr| 42 - 28]
+def e11 :  Expr Γ Ty.bool := `[Expr| (10 + 4 < 15 - 1) && (42 = 28 + x) && b]
+
+def example1 : Com Γ := `[Com|
   x := 8;
   y := 10;
   if (x < y) {
@@ -100,7 +143,7 @@ def example1 := `[Com|
   }]
 #reduce example1
 
-def example2 := `[Com|
+def example2 : Com Γ := `[Com|
   x := 8;
   if (x < y) {
     x := x + 1;
@@ -111,7 +154,7 @@ def example2 := `[Com|
   y := x;]
 #reduce example2
 
-def example3 := `[Com|
+def example3 : Com Γ := `[Com|
   if (x < 10) {
     x := 8;
   } else {
@@ -122,7 +165,7 @@ def example3 := `[Com|
   }]
 #reduce example3
 
-def example4 := `[Com|
+def example4 : Com Γ := `[Com|
   x := 13;
   y := 7;
   while (y = x - 5) {
@@ -130,4 +173,4 @@ def example4 := `[Com|
   }]
 #reduce example4
 
-end While
+end test
