git/g4rgoil/tba-project/TBA/While/Semantics.lean
@@ -2,58 +2,64 @@
 import TBA.While.Com
 
 namespace While
+
 open Com
 
-abbrev Map (α β : Type) := α → Option β
+abbrev State (Γ : Ctxt) := (τ : Ty) → (x : VName) → Γ x = some τ → Option (Val τ)
 
-namespace Map
+namespace State
 
-def empty : Map α β := fun k => none
+def empty : State Γ := λ _ _ _ => none
 
-def update [DecidableEq α] (m : Map α β) (k : α) (v : Option β) : Map α β :=
-  fun k' => if k = k' then v else m k'
+def update (m : State Γ) (x : VName) (_ : Γ x = some τ) (v : Option (Val τ))
+    : State Γ := λ τ' x' h' =>
+  if hτ : τ = τ' then (if x = x' then hτ ▸ v else m τ' x' h') else m τ' x' h'
 
-macro:max m:term noWs "[" k:term " ↦ " v:term "]" : term => `(update $m $k $v)
+def merge (m₁ : State Γ) (m₂ : State Γ) : State Γ := λ τ x h =>
+  if m₁ τ x h = m₂ τ x h then m₁ τ x h else none
 
-end Map
+-- Update syntax is extended to include proof of the variable's type
+scoped notation:max m "[" h " : " x " ↦ " v "]" => update m x h v
 
-abbrev State := Map VName Val
+end State
 
 namespace Expr
 
-variable (σ : State) in
-def eval : Expr → Option Val
-  | Expr.const v => some v
-  | Expr.var x   => σ x
-  | Expr.binop e₁ op e₂ => match eval e₁, eval e₂ with
-    | some v₁, some v₂ => op.eval v₁ v₂  -- BinOp.eval : BinOp → Val → Val → Option Val
+variable (σ : State Γ) in
+def eval : Expr Γ τ → Option (Val τ)
+  | Expr.const v => v
+  | Expr.var x h => σ τ x h
+  | Expr.binop e₁ op e₂ =>
+    match eval e₁, eval e₂ with
+    | some v₁, some v₂ => some (op.eval v₁ v₂)
     | _,       _       => none
 
-def time : Expr → Nat
-  | Expr.const v => 1
-  | Expr.var x   => 1
-  | Expr.binop e₁ op e₂ => time e₁ + time e₂ + 1
+def time : Expr Γ τ → Nat
+  | Expr.const _ => 1
+  | Expr.var _ _ => 1
+  | Expr.binop e₁ _ e₂ => time e₁ + time e₂ + 1
 
 end Expr
 
 open Expr
+open State
 
 section
 set_option hygiene false  -- HACK: allow forward reference in notation
 -- note the `local` to make the hacky notation local to the current section
 local notation:60 "⟨" c ", " σ "⟩"  " ⇓ " σ' " : " t:60 => Bigstep c σ σ' t
 
-inductive Bigstep : Com → State → State → Nat → Prop where
+inductive Bigstep : Com Γ → State Γ → State Γ → Nat → Prop where
   | skip :
     ⟨skip, σ⟩ ⇓ σ : 1
   | ass :
-    ⟨x ::= e, σ⟩ ⇓ σ[x ↦ e.eval σ] : e.time + 1
+    ⟨Com.ass x e h, σ⟩ ⇓ σ[h : x ↦ Expr.eval σ e] : e.time + 1
   | seq (h₁ : ⟨c₁, σ⟩ ⇓ σ' : t₁) (h₂ : ⟨c₂, σ'⟩ ⇓ σ'' : t₂) :
     ⟨c₁;; c₂, σ⟩ ⇓ σ'' : t₁ + t₂ + 1
   | ifTrue (hb : eval σ b = true) (ht : ⟨cₜ, σ⟩ ⇓ σ' : t) :
-    ⟨cond b cₜ cₑ, σ⟩ ⇓ σ' : b.time + t + 1
+    ⟨.cond b cₜ cₑ, σ⟩ ⇓ σ' : b.time + t + 1
   | ifFalse (hb : eval σ b = false) (he : ⟨cₑ, σ⟩ ⇓ σ' : t) :
-    ⟨cond b cₜ cₑ, σ⟩ ⇓ σ' : b.time + t + 1
+    ⟨.cond b cₜ cₑ, σ⟩ ⇓ σ' : b.time + t + 1
   | whileTrue (hb : eval σ b = true) (hc : ⟨c, σ⟩ ⇓ σ' : t₁) (hind : ⟨.while b c, σ'⟩ ⇓ σ'' : t₂) :
     ⟨.while b c, σ⟩ ⇓ σ'' : b.time + t₁ + t₂ + 1
   | whileFalse (hb : eval σ b = false) :
