git/g4rgoil/tba-project/TBA/While/Solution.lean
@@ -3,71 +3,56 @@ import TBA.While.Semantics
 import Aesop
 import TBA.Util.AesopExts
 
+
 namespace While
-
-section task1
-
-theorem deterministic: ⟨c,σ⟩ ⇓ σ₁ : t₁ → ⟨c, σ⟩ ⇓ σ₂ : t₂ → t₁ = t₂ ∧ σ₁ = σ₂ := by
-  intro h1 h2
-  induction h1 generalizing σ₂ t₂ with
-  | skip => cases h2 <;> simp
-  | ass => cases h2 <;> simp
-  | seq _ _ ih₁ ih₂ => cases h2 with | seq hc1 hc2 => 
-    have h := ih₁ hc1
-    rw[And.right h] at ih₂
-    have h' := ih₂ hc2
-    simp_all
-  | ifTrue _ _ ih | ifFalse _ _ ih => cases h2 <;> simp_all [ih (by assumption)]
-  | whileTrue hexpr _ _ ih₁ ih₂ => 
-    cases h2 with 
-    | whileFalse => simp_all
-    | whileTrue _ hc₁' hw' =>
-      have h := ih₁ hc₁'
-      rw[And.right h] at ih₂
-      have h' := ih₂ hw'
-      simp_all
-  | whileFalse => cases h2 <;> simp_all
-
-end task1
-
-namespace Optimisation
-
-
-
+open State
 
 -- Task 1: The semantic is deterministic.
 section task_1
--- TODO
-theorem semDeterministic : ⟨c, σ⟩ ⇓ σ₁ : t₁ → ⟨c, σ⟩ ⇓ σ₂ : t₂ → ((∀ x, σ₁ x = σ₂ x) ∧  t₁ = t₂) := by
-  sorry
+
+theorem BigstepDeterministic (h₁ : ⟨c, σ⟩ ⇓ σ₁ : t₁) (h₂ : ⟨c, σ⟩ ⇓ σ₂ : t₂)
+    : σ₁ = σ₂ ∧ t₁ = t₂ := by
+  induction h₁ generalizing σ₂ t₂ with
+  | skip | ass => cases h₂ <;> trivial
+  | seq _ _ ih₁ ih₂ =>
+    cases h₂ with
+    | seq hc₁ hc₂ =>
+      have ⟨hσ, _⟩ := ih₁ hc₁
+      simp_all [(hσ ▸ ih₂) hc₂]
+  | ifTrue _ _ ih | ifFalse _ _ ih => cases h₂ <;> simp_all [ih ‹_›]
+  | whileTrue _ _ _ ihc ihind =>
+    cases h₂ with
+    | whileTrue _ hc hind =>
+      have ⟨hσ, _⟩ := ihc hc
+      simp_all [(hσ ▸ ihind) hind]
+    | whileFalse => simp_all
+  | whileFalse => cases h₂ <;> simp_all
+
 end task_1
 
 
-
+namespace Optimisation
 
 -- Task 2: Formalisation of constant propagation and folding
 section task_2
 
-def foldExpr (σ : State) : Expr → Expr
+def foldExpr (σ : State Γ) : Expr Γ τ → Expr Γ τ
   | .const v => Expr.const v
-  | .var x =>
-    match σ x with
+  | .var x h =>
+    match σ _ x h with
     | some v => Expr.const v
-    | none   => Expr.var x
+    | none   => Expr.var x h
   | .binop e₁ op e₂ =>
     match foldExpr σ e₁, foldExpr σ e₂ with
-    | .const v₁, .const v₂ =>
-      match op.eval v₁ v₂ with
-      | some v => Expr.const v
-      | none   => Expr.binop v₁ op v₂
-    | e₁', e₂' => Expr.binop e₁' op e₂'
+    | .const v₁, .const v₂ => Expr.const (op.eval v₁ v₂)
+    | e₁',       e₂'       => Expr.binop e₁' op e₂'
 
-def foldCom (σ : State) : Com → (Com × State)
+def foldCom (σ : State Γ) : Com Γ → (Com Γ × State Γ)
   | .skip => (Com.skip, σ)
-  | .ass x e =>
+  | .ass x e h =>
       match foldExpr σ e with
-      | .const v => (Com.ass x v, σ[x ↦ v])
-      | e'       => (Com.ass x e', σ[x ↦ none])
+      | .const v => (Com.ass x v h, σ[h : x ↦ v])
+      | e'       => (Com.ass x e' h, σ[h : x ↦ none])
   | .seq c₁ c₂ =>
     have (c₁', σ')  := foldCom σ c₁
     have (c₂', σ'') := foldCom σ' c₂
@@ -78,237 +63,183 @@ def foldCom (σ : State) : Com → (Com × State)
     | .const false => foldCom σ cₑ
     | b' =>
       have ((cₜ', σₜ), (cₑ', σₑ)) := (foldCom σ cₜ, foldCom σ cₑ)
-      (Com.cond b' cₜ' cₑ', λ k => if σₜ k = σₑ k then σₜ k else none)
+      (Com.cond b' cₜ' cₑ', merge σₜ σₑ)
   | .while b c =>
     match foldExpr σ b with
     | .const false => (Com.skip, σ)
-    | _            => (Com.while b (foldCom Map.empty c).1, Map.empty)
+    | _            => (Com.while b (foldCom empty c).1, empty)
 
-def optimise : Com → Com := λ c => (foldCom Map.empty c).1
-
-
-theorem Expr.custom_rec (p : Expr → Prop)
-    (htrue : p true) (hfalse : p  false) (hint : ∀ (x : Int), p x)
-    (hvar : ∀ (x : VName), p x) (hbinop : ∀ l op r, p (Expr.binop l op r))
-    : ∀ v, p v
-  | true | false | Val.int _ | .var _ | .binop .. => by simp_all
+def optimise : Com Γ → Com Γ := λ c => (foldCom empty c).1
 
 end task_2
 
 
+section task_3_and_4
 
+attribute [local simp] foldExpr Nat.add_le_add Nat.le_add_left Nat.le_refl
 
--- Task 3: The optimisation preserves the semantics of a program.
-section task_3
+-- Necessary relation between any optimisation and evaluation state of a program.
+-- In short: The optimisation state (ρ) must be a subset of the evaluation state (σ).
+abbrev ConstMap {Γ : Ctxt} (σ ρ : State Γ) :=
+  ∀ (τ : Ty) (x : VName) (h : Γ x = some τ) (v : Val τ),
+    ρ τ x h = some v → σ τ x h = some v
 
-abbrev ConstMap (σ ρ : State) := ∀ x v, ρ x = some v → σ x = some v
-
-variable {c : Com} {e : Expr} {σ σ' ρ : State} {t : Nat}
-
-attribute [local simp] foldExpr
-
-theorem empty_ConstMap : ConstMap σ Map.empty := by
-  intro _ _ _; trivial
+theorem empty_ConstMap : ConstMap σ empty := by
+  intro _ _ _ _ _; trivial
 
 theorem foldExprSound (h : ConstMap σ ρ) : Expr.eval σ e = Expr.eval σ (foldExpr ρ e) := by
-  induction e <;> aesop (add norm unfold Expr.eval)
+  induction e with
+    rw [foldExpr]
+  | var                 => aesop
+  | binop _ _ _ ihl ihr =>
+    aesop (add norm unfold Expr.eval, safe forward ihl, safe forward ihr)
 
 theorem foldCom_ConstMap (h : ConstMap σ ρ) (hc : ⟨c, σ⟩ ⇓ σ' : t)
     : ConstMap σ' (foldCom ρ c).2 := by
   induction hc generalizing ρ with
     simp only [foldCom]
   | skip => exact h
-  | ass => intro; aesop (add norm unfold Map.update, safe forward foldExprSound)
+  | ass =>
+    intro _ _ _ _
+    aesop (add norm unfold State.update, safe forward foldExprSound)
   | seq _ _ ih₁ ih₂ => exact ih₂ (ih₁ h)
-  | ifTrue _ _ ih | ifFalse _ _ ih =>
-    cases hfold : foldExpr ρ ‹Expr› using Expr.custom_rec with
+  | @ifTrue _ b _ _ _ _ _ _ ih | @ifFalse _ b _ _ _ _ _ _ ih =>
+    cases hfold : foldExpr ρ b using Expr.bool_rec with
     | htrue | hfalse =>
       first | exact ih h | simp_all [foldExprSound h, Expr.eval]
-    | _ => intro _ _ _; rw [ih h]; aesop
-  | whileTrue =>
-    cases hfold : foldExpr ρ ‹Expr› using Expr.custom_rec with
+    | _ =>
+      intro _ _ _ _ _
+      apply ih h
+      aesop (add norm unfold State.merge)
+  | @whileTrue _ b =>
+    cases hfold : foldExpr ρ b using Expr.bool_rec with
     | hfalse => simp_all [foldExprSound h, Expr.eval]
     | _      => exact empty_ConstMap
   | whileFalse => split <;> first | exact h | exact empty_ConstMap
 
-theorem foldExprEmpty (hfold : foldExpr Map.empty e = Expr.const v)
+theorem foldExprEmpty (hfold : foldExpr empty e = Expr.const v)
     : foldExpr σ e = Expr.const v := by
-  induction e generalizing v with
-  | const => rw [←hfold]; rfl
-  | var x => simp_all [Map.empty]
+  induction e with
+  | const => exact hfold
+  | var   => contradiction
   | binop l op r ihl ihr =>
-    match hl : foldExpr Map.empty l, hr : foldExpr Map.empty r with
+    match hl : foldExpr empty l, hr : foldExpr empty r with
     | .const _, .const _ => simp_all [ihl hl, ihr hr]
-    | .var _, _ | _, .var _ | .binop .., _ | _, .binop .. => simp_all
+    | .var .., _ | _, .var .. | .binop .., _ | _, .binop .. => simp_all
+
+theorem foldExprTime : (Expr.time (foldExpr ρ e)) ≤ (Expr.time e) := by
+  induction e <;> aesop (add norm unfold Expr.time)
+
+theorem foldComSoundTime (h : ConstMap σ ρ) (hc : ⟨c, σ⟩ ⇓ σ' : t)
+    : ∃ t', ⟨(foldCom ρ c).1, σ⟩ ⇓ σ' : t' ∧ t' ≤ t := by
+  induction hc generalizing ρ with
+    simp only [foldCom]
+  | skip => exact ⟨_, Bigstep.skip, Nat.le_refl _⟩
+  | @ass _ _ e =>
+    rw [foldExprSound h]
+    cases hfold : foldExpr ρ e with
+    | _ => exact ⟨_, Bigstep.ass, by simp_all [hfold ▸ foldExprTime]⟩
+  | seq hc₁ _ ih₁ ih₂ =>
+    have ⟨_, h₁, _⟩ := ih₁ h
+    have ⟨_, h₂, _⟩ := ih₂ (foldCom_ConstMap h hc₁)
+    exact ⟨_, Bigstep.seq h₁ h₂, by simp_all⟩
+  | @ifTrue _ b _ _ _ _ hb _ ih | @ifFalse _ b _ _ _ _ hb _ ih =>
+    cases hfold : foldExpr ρ b using Expr.bool_rec with
+    | htrue | hfalse =>
+      have ⟨_, hc, hle⟩ := ih h
+      first | exact ⟨_, hc, Nat.le_step (Nat.le_trans hle (Nat.le_add_left ..))⟩
+            | simp_all [foldExprSound h, Expr.eval]
+    | _ =>
+      rw [foldExprSound h, hfold] at hb
+      have ⟨_, hc, _⟩ := ih h
+      first | refine ⟨_, Bigstep.ifTrue hb hc, ?_⟩
+            | refine ⟨_, Bigstep.ifFalse hb hc, ?_⟩
+      simp_all [hfold ▸ foldExprTime]
+  | @whileTrue _ b _ _ _ _ _ hb _ _ ihc ihind =>
+    cases hfold : foldExpr ρ b using Expr.bool_rec with
+    | hfalse => simp_all [foldExprSound h, Expr.eval]
+    | _ =>
+      cases hfold' : foldExpr empty b using Expr.bool_rec with
+      | hfalse => simp_all [foldExprEmpty hfold']
+      | _ =>
+        have ⟨_, hc, _⟩ := ihc empty_ConstMap
+        have ⟨_, hind, _⟩ := ihind empty_ConstMap
+        rw [foldCom, hfold'] at hind
+        refine ⟨_, Bigstep.whileTrue hb hc hind, ?_⟩
+        apply Nat.add_le_add_right <;> simp_all
+  | @whileFalse _ b _ hb =>
+    cases foldExpr ρ b using Expr.bool_rec with
+    | hfalse => exact ⟨_, Bigstep.skip, Nat.le_add_left _ _⟩
+    | _      => exact ⟨_, Bigstep.whileFalse hb, Nat.le_refl _⟩
+
+end task_3_and_4
+
+
+-- Task 3: The optimisation preserves the semantics of a program.
+section task_3
 
 theorem foldComSound (h : ConstMap σ ρ) (hc : ⟨c, σ⟩ ⇓ σ' : t)
     : ∃ t', ⟨(foldCom ρ c).1, σ⟩ ⇓ σ' : t' := by
-  induction hc generalizing ρ with
-    simp only [foldCom]
-  | skip => exact ⟨1, Bigstep.skip⟩
-  | ass =>
-    rw [foldExprSound h]
-    cases foldExpr ρ ‹Expr› <;> exact ⟨_, Bigstep.ass⟩
-  | seq hc₁ _ ih₁ ih₂ =>
-    match ih₁ h, ih₂ (foldCom_ConstMap h hc₁) with
-    | ⟨_, h₁⟩, ⟨_, h₂⟩ => exact ⟨_, Bigstep.seq h₁ h₂⟩
-  | ifTrue hb _ ih | ifFalse hb _ ih =>
-    cases hfold : foldExpr ρ ‹Expr› using Expr.custom_rec with
-    | htrue | hfalse =>
-      first | exact ih h | simp_all [foldExprSound h, Expr.eval]
-    | _ =>
-      rw [foldExprSound h, hfold] at hb
-      have ⟨_, hc⟩ := ih h
-      first | exact ⟨_, Bigstep.ifTrue hb ‹_›⟩
-            | exact ⟨_, Bigstep.ifFalse hb ‹_›⟩
-  | whileTrue hb _ _ ihc ihind =>
-    rename Expr => b
-    cases hfold : foldExpr ρ b using Expr.custom_rec with
-    | hfalse => simp_all [foldExprSound h, Expr.eval]
-    | _ =>
-      cases hfold' : foldExpr Map.empty b using Expr.custom_rec with
-      | hfalse => simp_all [foldExprEmpty hfold']
-      | _ =>
-        have ⟨_, hc⟩ := ihc empty_ConstMap
-        have ⟨_, hind⟩ := ihind empty_ConstMap
-        rw [foldCom, hfold'] at hind
-        exact ⟨_, Bigstep.whileTrue hb hc hind⟩
-  | whileFalse hb =>
-    cases foldExpr ρ ‹Expr› using Expr.custom_rec with
-    | hfalse => exact ⟨_, Bigstep.skip⟩
-    | _      => exact ⟨_, Bigstep.whileFalse hb⟩
+  have ⟨t', hc', _ ⟩ := foldComSoundTime h hc
+  exact ⟨t', hc'⟩
 
--- Main prove that the constant propagation is sound (Task 3)
-theorem optimiseSound : ⟨c, σ⟩ ⇓ σ' : t → ∃ t', ⟨optimise c, σ⟩ ⇓ σ' : t' := 
+-- Main prove that the constant propagation is sound
+theorem optimiseSound : ⟨c, σ⟩ ⇓ σ' : t → ∃ t', ⟨optimise c, σ⟩ ⇓ σ' : t' :=
   foldComSound empty_ConstMap
 
 end task_3
 
 
-
-
 -- Task 4: The optimisation does not increase execution time.
 section task_4
 
-open Nat
-
-variable {c : Com} {e : Expr} {σ σ' ρ : State} {t t₁ t₂ : Nat}
-
-attribute [local simp] foldExpr
-attribute [local simp] Nat.le_add_left Nat.le_refl Nat.add_le_add_right Nat.add_le_add_left Nat.add_le_add Nat.zero_le
-
-
--- TODO: Make nicer
-theorem foldExprTime : (Expr.time (foldExpr σ e)) ≤ (Expr.time e) := by
-  induction e with simp only [foldExpr, Expr.time]
-  | var x => split <;> simp only [Expr.time]
-  | binop e₁ op e₂ h₁ h₂ =>
-    cases a : foldExpr σ e₁ with simp_all [Expr.time, add_le_add]
-    | const v₁ =>
-      cases b : foldExpr σ e₂ with simp_all [Expr.time, add_le_add]
-      | const v₂ =>
-        split
-        simp only [Expr.time, Nat.le_add_left 1 _]
-        simp only [Expr.time]
-        exact (Nat.add_le_add_right (Nat.add_le_add h₁ h₂) 1)
-
-theorem foldCom_SoundTime (h : ConstMap σ ρ) (hc : ⟨c, σ⟩ ⇓ σ' : t)
-    : ∃ t', ⟨(foldCom ρ c).1, σ⟩ ⇓ σ' : t' ∧ t' ≤ t := by
-  induction hc generalizing ρ with
-    simp only [foldCom]
-  | skip => exact ⟨1, ⟨Bigstep.skip, Nat.le_refl 1⟩⟩
-  | ass =>
-    rw [foldExprSound h]
-    cases e' : foldExpr ρ ‹Expr› <;> exact ⟨_, ⟨Bigstep.ass, Nat.add_le_add_right (e' ▸ foldExprTime) 1⟩⟩
-  | seq hc₁ _ ih₁ ih₂ =>
-    match ih₁ h, ih₂ (foldCom_ConstMap h hc₁) with
-    | ⟨t₁, ⟨h₁, le₁⟩⟩, ⟨t₂, ⟨h₂, le₂⟩⟩ =>
-      have le := Nat.add_le_add_right (Nat.add_le_add le₁ le₂) 1
-      exact ⟨t₁ + t₂ + 1, ⟨Bigstep.seq h₁ h₂, le⟩⟩
-  | ifTrue hb _ ih | ifFalse hb _ ih =>
-    rename Expr => b
-    cases hfold : foldExpr ρ ‹Expr› using Expr.custom_rec with
-    | htrue | hfalse =>
-      have ⟨w, ⟨hw, hle⟩⟩ := ih h
-      have le := Nat.add_le_add (Nat.add_le_add (Nat.zero_le (Expr.time b)) hle) (Nat.zero_le 1)
-      simp at le
-      first | exact ⟨w, ⟨hw, le⟩⟩
-            | simp_all [ih h, foldExprSound h, foldExprTime, Expr.eval]
-    | _ =>
-      rw [foldExprSound h, hfold] at hb
-      have ⟨w, ⟨hw, hle⟩⟩ := ih h
-      have le : Expr.time (foldExpr ρ b) + w + 1 ≤ Expr.time b + _ + 1 := Nat.add_le_add (Nat.add_le_add foldExprTime hle) (Nat.le_refl 1)
-      rw [hfold] at le
-      first | exact ⟨_, ⟨Bigstep.ifTrue hb hw, le⟩⟩
-            | exact ⟨_, ⟨Bigstep.ifFalse hb hw, le⟩⟩
-  | whileTrue hb _ _ ihc ihind =>
-    rename Expr => b
-    cases hfold : foldExpr ρ b using Expr.custom_rec with
-    | hfalse => simp_all [foldExprSound h, Expr.eval]
-    | _ =>
-      cases hfold' : foldExpr Map.empty b using Expr.custom_rec with
-      | hfalse => simp_all [foldExprEmpty hfold']
-      | _ =>
-        have ⟨hct, hc⟩ := ihc empty_ConstMap
-        have ⟨hindt, hind⟩ := ihind empty_ConstMap
-        rw [foldCom, hfold'] at hind
-        simp at hind
-        have le := Nat.add_le_add (Nat.add_le_add (Nat.add_le_add (Nat.le_refl (Expr.time b)) hc.2) hind.2) (Nat.le_refl 1)
-        exact ⟨_, ⟨Bigstep.whileTrue hb hc.1 hind.1, le⟩⟩
-  | whileFalse hb =>
-    cases foldExpr ρ ‹Expr› using Expr.custom_rec with
-    | hfalse => exact ⟨_, ⟨Bigstep.skip, by simp⟩⟩
-    | _      => exact ⟨_, ⟨Bigstep.whileFalse hb, Nat.le_refl _⟩⟩
-
-
-theorem optimise_SoundTime : ⟨c, σ⟩ ⇓ σ' : t → ∃ t', ⟨optimise c, σ⟩ ⇓ σ' : t' ∧ t' ≤ t := 
-  foldCom_SoundTime empty_ConstMap
-
-
-theorem optimiseTime (h₁ : ⟨c, σ⟩ ⇓ σ' : t₁) (h₂ : ⟨optimise c, σ⟩ ⇓ σ' : t₂) : t₂ ≤ t₁ := by
-  have ⟨_, ⟨h₂', leq⟩⟩ := optimise_SoundTime h₁
-  have ⟨eq, _⟩ := deterministic h₂ h₂'
-  exact eq ▸ leq
+theorem optimiseTime (h₁ : ⟨c, σ⟩ ⇓ σ' : t₁) (h₂ : ⟨optimise c, σ⟩ ⇓ σ'' : t₂) : t₂ ≤ t₁ := by
+  have ⟨_, h₂', hle⟩ := foldComSoundTime empty_ConstMap h₁
+  have ⟨_, heq⟩ := BigstepDeterministic h₂ h₂'
+  exact heq ▸ hle
 
 end task_4
 
 
-
-
--- Task 5: Constant propagation is idempotent.
+-- Task 5: The optimisation is idempotent.
 section task_5
 
-attribute [local simp] foldExpr
-attribute [local simp] foldCom
-
 theorem foldExprIdempotent : foldExpr σ (foldExpr σ e) = foldExpr σ e := by
-  induction e <;> aesop
+  induction e <;> aesop (add norm unfold foldExpr)
 
-attribute [local simp] foldExprIdempotent
+theorem foldComIdempotent : foldCom σ (foldCom σ c).1 = foldCom σ c := by
+  induction c generalizing σ with
+    simp only [foldCom]
+  | ass _ e =>
+    cases hfold : foldExpr σ e with
+    | const => rw [foldCom, foldExpr]
+    | _     => rw [foldCom, ←hfold, foldExprIdempotent]
+  | seq _ _ ihl ihr => rw [ihl, ihr]
+  | cond b =>
+    cases hfold : foldExpr σ b using Expr.bool_rec with
+    | htrue | hfalse => simp_all
+    | _ =>
+      rw [foldCom, ←hfold, foldExprIdempotent]
+      simp_all
+  | «while» => split <;> simp_all [foldCom]
 
-
--- TODO: Finalize proof
-theorem foldComIdempotent : foldCom σ ((foldCom σ c).1) = foldCom σ c := by
-  sorry
-
-
+-- Main prove that the constant propagation is idempotent (Task 5)
 theorem optimiseIdempotent : optimise (optimise c) = optimise c := by
-  simp_all [optimise]; aesop (add norm foldComIdempotent)
+  unfold optimise
+  exact congrArg _ foldComIdempotent
 
 end task_5
 
 
-
-
--- Task 6: Formalize typing
 section task_6
+
+-- Nothing to prove here:
+-- 1) Only well-typed Expressions and Programs can be instantiated.
+-- 2) Therefore `foldExpr` and `foldCom` may only return well-typed Expressions
+--    and Programs by definition. The same also applies to `optimise`.
 
 end task_6
 
-
-
-
 end Optimisation
-
 
 end While
